<?xml version="1.0" encoding="UTF-8"?>

<!DOCTYPE rdf:RDF [
  <!ENTITY owl "http://www.w3.org/2002/07/owl#">
  <!ENTITY rdf "http://www.w3.org/1999/02/22-rdf-syntax-ns#">
  <!ENTITY rdfs "http://www.w3.org/2000/01/rdf-schema#">
  <!ENTITY xsd "http://www.w3.org/2001/XMLSchema#">
]>

<rdf:RDF 
         xmlns:owl="&owl;"    
         xmlns:rdf="&rdf;"
         xmlns:rdfs="&rdfs;"
		 xmlns:xsd = "&xsd;">

<!-- Ontology Information -->
  <owl:Ontology rdf:about=""
                owl:versionInfo="2.0">
  </owl:Ontology>
  
	<owl:Class rdf:ID="Thunderstorm"/>
	<owl:Class rdf:ID="ElectricPotential"/>
	<owl:Class rdf:ID="Sound"/>
 
  <owl:Class rdf:ID="BallLightning">
    <rdfs:subClassOf rdf:resource="#Lightning" />
    <rdfs:comment xml:lang="en">A rare and randomly occurring bright ball of light observed floating or moving through the atmosphere close to the ground.
    </rdfs:comment>
  </owl:Class>

  <owl:Class rdf:ID="BeadedLightning">
    <rdfs:subClassOf rdf:resource="#Lightning" />
    <rdfs:comment xml:lang="en">A particular aspect of a normal lightning flash occasionally seen when the observer happens to view end-on a number of segments of the irregular channel (zigzag lightning) and hence receives an impression of higher luminosity at a series of locations along the channel.</rdfs:comment>
  </owl:Class>

  <owl:Class rdf:ID="BlueJet">
    <rdfs:subClassOf rdf:resource="#Lightning" />
    <rdfs:comment xml:lang="en">Weakly luminous upward propagating discharges, blue in color, emanating from the tops of thunderstorms.
    </rdfs:comment>
  </owl:Class>

  <owl:Class rdf:ID="JunctionStreamer">
    <rdfs:subClassOf>
      <owl:Restriction>
		<owl:onProperty>		
		<owl:ObjectProperty rdf:ID="hasMeteorologicalPhenomena"/>	
		</owl:onProperty>
        <owl:allValuesFrom rdf:resource="#Thunderstorm" />
      </owl:Restriction>
    </rdfs:subClassOf>
    <rdfs:subClassOf>
      <owl:Restriction>
        <owl:onProperty rdf:resource="#hasMeteorologicalPhenomena" />
        <owl:allValuesFrom rdf:resource="#Lightning" />
     </owl:Restriction>
    </rdfs:subClassOf>
    <rdfs:subClassOf rdf:resource="#Lightning" />
    <rdfs:comment xml:lang="en">The process by which negative charge centers at successively more distant locations in a thundercloud are tapped for discharge by successive strokes of cloud-to-ground lightning.</rdfs:comment>
  </owl:Class>

  <owl:Class rdf:ID="Lightning">
    <rdfs:subClassOf rdf:resource="#MeteorologicalPhenomena"/>
    <rdfs:subClassOf>
      <owl:Restriction>
		<owl:onProperty>		
		<owl:ObjectProperty rdf:ID="hasPhysicalProcess"/>	
		</owl:onProperty>
        <owl:someValuesFrom rdf:resource="#ElectricPotential" />
     </owl:Restriction>
    </rdfs:subClassOf>
    <rdfs:subClassOf>
      <owl:Restriction>
        <owl:onProperty rdf:resource="#hasMeteorologicalPhenomena" />
        <owl:allValuesFrom rdf:resource="#Thunder" />
       </owl:Restriction>
    </rdfs:subClassOf>
    <rdfs:comment xml:lang="en">Lightning is a transient, high-current electric discharge with pathlengths measured in kilometers. The most common source of lightning is the electric charge separated in ordinary thunderstorm clouds.   
    </rdfs:comment>
  </owl:Class>

  <owl:Class rdf:ID="ReturnStroke">
    <rdfs:subClassOf rdf:resource="#Lightning" />
    <rdfs:comment xml:lang="en">The intense luminosity that propagates upward from earth to cloud base in the last phase of each lightning stroke of a cloud-to-ground discharge.</rdfs:comment>
  </owl:Class>

  <owl:Class rdf:ID="Thunder">
    <rdfs:subClassOf rdf:resource="#MeteorologicalPhenomena" />
    <rdfs:subClassOf rdf:resource="#Sound" />
    <rdfs:comment xml:lang="en">The sound emitted by rapidly expanding gases along the channel of a lightning discharge.
    </rdfs:comment>
  </owl:Class>

</rdf:RDF>
