<?xml version="1.0" encoding="UTF-8"?>

<!DOCTYPE rdf:RDF [
  <!ENTITY owl "http://www.w3.org/2002/07/owl#">
  <!ENTITY rdf "http://www.w3.org/1999/02/22-rdf-syntax-ns#">
  <!ENTITY rdfs "http://www.w3.org/2000/01/rdf-schema#">
  <!ENTITY xsd "http://www.w3.org/2001/XMLSchema#">
]>

<rdf:RDF 
         xmlns:owl="&owl;"    
         xmlns:rdf="&rdf;"
         xmlns:rdfs="&rdfs;"
		 xmlns:xsd = "&xsd;">

<!-- Ontology Information -->
  <owl:Ontology rdf:about=""
                owl:versionInfo="2.0">
  </owl:Ontology>

<!-- Classes -->
  <owl:Class rdf:ID="GeologicFeature"/>
  <owl:Class rdf:ID="Depression"/>
  <owl:Class rdf:ID="Molasse"/>
  
  <owl:Class rdf:ID="BackArcBasin">
    <rdfs:subClassOf rdf:resource="#Basin"/>
    <rdfs:comment xml:lang="en">Back-arc basins (or retro-arc basins) are geologic features, submarine basins associated with island arcs and subduction zones. They are found at some convergent plate boundaries, presently concentrated in the Western Pacific ocean. [Wikipedia]</rdfs:comment>
  </owl:Class>

   <owl:Class rdf:ID="Basin">
    <rdfs:subClassOf rdf:resource="#GeologicFeature"/>
    <rdfs:subClassOf rdf:resource="#Depression"/>
  </owl:Class>

  <owl:Class rdf:ID="FlyschBasin">
    <rdfs:subClassOf rdf:resource="#Basin"/>
    <rdfs:comment xml:lang="en">Flysch is a sequence of sedimentary rocks that is deposited in a deep marine facies in the foreland basin of a developing orogen. Flysch is formed under deep marine circumstances, in a quiet and low-energetic depositional environment. [Wikipedia]</rdfs:comment>
  </owl:Class>

  <owl:Class rdf:ID="ForelandBasin">
    <rdfs:subClassOf rdf:resource="#Basin"/>
    <rdfs:comment xml:lang="en">A foreland basin is a depression that develops adjacent and parallel to a mountain belt. Foreland basins form because the immense mass created by crustal thickening associated with the evolution of a mountain belt causes the lithosphere to bend, by a process known as lithospheric flexure. [Wikipedia]</rdfs:comment>
  </owl:Class>

  <owl:Class rdf:ID="ForeArcBasin">
    <rdfs:subClassOf rdf:resource="#Basin"/>
    <rdfs:comment xml:lang="en">A forearc is a depression (basin) in the sea floor located between a subduction zone and an associated volcanic arc. It is typically filled with sediments from the adjacent landmass and the island arc in addition to trapped oceanic crustal material. [Wikipedia]</rdfs:comment>
  </owl:Class>

  <owl:Class rdf:ID="IntracratonicBasin">
    <rdfs:subClassOf rdf:resource="#Basin"/>
    <rdfs:comment xml:lang="en">Intracratonic basins are formed by fluvial sedimentation of an intracratonic area which has undergone sediment sag-loading. [Wikipedia]</rdfs:comment>
  </owl:Class>

   <owl:Class rdf:ID="IntraArcBasin">
    <rdfs:subClassOf rdf:resource="#Basin"/>
    <rdfs:comment xml:lang="en">Intra-arc basins are basins that occur between Fore-arc basins and back-arc basins [Wikipedia]</rdfs:comment>
  </owl:Class>

  <owl:Class rdf:ID="PeripheralForelandBasin">
    <rdfs:subClassOf rdf:resource="#Basin"/>
    <rdfs:subClassOf>
      <owl:Restriction>
        <owl:allValuesFrom rdf:resource="#Molasse"/>
		<owl:onProperty>		
		<owl:ObjectProperty rdf:ID="hasSubstance"/>	
		</owl:onProperty>
      </owl:Restriction>
    </rdfs:subClassOf>
    <rdfs:subClassOf>
      <owl:Restriction>
		<owl:onProperty>		
		<owl:ObjectProperty rdf:ID="hasPlanetaryStructure"/>	
		</owl:onProperty>
        <owl:allValuesFrom rdf:resource="#FlyschBasin"/>
      </owl:Restriction>
    </rdfs:subClassOf>
    <rdfs:comment xml:lang="en">Peripheral (Pro) foreland basins occur on the plate that is subducted or underthrust during plate collision (i.e. the outer arc of the orogen).</rdfs:comment>
  </owl:Class>

  <owl:Class rdf:ID="SuccessorBasin">
    <rdfs:subClassOf rdf:resource="#Basin"/>
    <rdfs:comment xml:lang="en">Successor basins arise from shifting and merging of fore arc, back-arc and intra-arc basins. Basins or sequences that overlap terrane boundaries. [Wikipedia]</rdfs:comment>
  </owl:Class>

  <owl:Class rdf:ID="RetroarcForelandBasin">
    <rdfs:subClassOf rdf:resource="#Basin"/>
    <rdfs:comment xml:lang="en">Retroarc (Retro) foreland basins occur on the plate that overrides during plate convergence or collision (i.e. situated behind the magmatic arc that is linked with the subduction of oceanic lithosphere). [Wikipedia]</rdfs:comment>
  </owl:Class>

  <owl:Class rdf:ID="TranstensionalBasin">
    <rdfs:subClassOf rdf:resource="#Basin"/>
    <rdfs:comment xml:lang="en">Transtension basins are oblique tensional environments where stretching takes place. [Wikipedia]</rdfs:comment>
  </owl:Class>

  <owl:Class rdf:ID="TranspressionalBasin">
    <rdfs:subClassOf rdf:resource="#Basin"/>
    <rdfs:comment xml:lang="en">Transpression basins are formed during oblique collision of tectonic plates and during non-orthogonal subduction. [Wikipedia]</rdfs:comment>
  </owl:Class>

   <owl:ObjectProperty rdf:ID="hasBasin">
    <rdfs:range rdf:resource="#Basin"/>
  </owl:ObjectProperty>

</rdf:RDF>
